progs/verif1.v
@@ -28,13 +28,13 @@ reflexivity.
 econstructor; simpl; reflexivity.
 Defined.
 
-Definition ilseg (s: list int) := lseg P.t_listptr (map Vint s).
+Definition ilseg (sh: share) (s: list int) := lseg P.t_listptr sh (map Vint s).
 
 Definition ilseg_nil (l: list  int) x z : mpred := !! (ptr_eq x z) && !! (l=nil) && emp.
-Definition ilseg_cons (s: list int) := lseg_cons P.t_listptr (map Vint s).
+Definition ilseg_cons (sh: share) (s: list int) := lseg_cons P.t_listptr sh (map Vint s).
 
-Lemma ilseg_unroll: forall l x z , 
-    ilseg l x z = ilseg_nil l x z || ilseg_cons l x z.
+Lemma ilseg_unroll: forall sh l x z , 
+    ilseg sh l x z = ilseg_nil l x z || ilseg_cons sh l x z.
 Proof.
 intros.
 unfold ilseg at 1.
@@ -46,18 +46,18 @@ f_equal.
 apply prop_ext; split; intro; destruct l; simpl in *; congruence.
 Qed.
 
-Lemma ilseg_eq: forall s p, 
+Lemma ilseg_eq: forall sh s p, 
    typecheck_val p P.t_listptr = true -> 
-    (ilseg s p p = !!(s=nil) && emp).
+    (ilseg sh s p p = !!(s=nil) && emp).
 Proof. intros. unfold ilseg. rewrite lseg_eq; auto. f_equal. f_equal.
  apply prop_ext. destruct s; simpl; intuition congruence.
 Qed.
 Hint Rewrite ilseg_eq : normalize.
 
 Lemma ilseg_nonnull:
-  forall s v,
+  forall sh s v,
       typed_true P.t_listptr v ->
-     ilseg s v nullval = ilseg_cons s v nullval.
+     ilseg sh s v nullval = ilseg_cons sh s v nullval.
 Proof.
 intros. subst. 
 rewrite ilseg_unroll.
@@ -76,7 +76,7 @@ rewrite H0 in H; inv H.
 normalize.
 Qed.
 
-Lemma ilseg_nil_eq: forall p q, ilseg nil p q = !! (ptr_eq p q) && emp.
+Lemma ilseg_nil_eq: forall sh p q, ilseg sh nil p q = !! (ptr_eq p q) && emp.
 Proof. intros.
  rewrite ilseg_unroll.
  apply pred_ext.
@@ -88,14 +88,14 @@ Qed.
 Hint Rewrite ilseg_nil_eq : normalize.
 
 Lemma lift2_ilseg_cons: 
- forall s p q, lift2 (ilseg_cons s)  p q =
+ forall sh s p q, lift2 (ilseg_cons sh s)  p q =
     EX hry:(int * list int * val),
       match hry with (h,r,y) =>
        !! (s = h::r) &&
        (local (lift2 ptr_neq p q) &&
-       (lift2 (field_mapsto Share.top list_struct list_data) p (lift0 (Vint h)) *
-        lift2 (field_mapsto Share.top list_struct list_link) p (lift0 y) *
-        |> lift2 (ilseg r) (lift0 y) q))
+       (lift2 (field_mapsto sh list_struct list_data) p (lift0 (Vint h)) *
+        lift2 (field_mapsto sh list_struct list_link) p (lift0 y) *
+        |> lift2 (ilseg sh r) (lift0 y) q))
      end.
 Proof.
  intros.
@@ -109,8 +109,8 @@ Proof.
  apply exp_right with (Vint h). normalize. apply exp_right with (map Vint r).
  normalize. apply exp_right with y. normalize.
  apply andp_right.
- forget (field_mapsto Share.top list_struct P.i_h (p rho) (Vint h) ) as A.
- forget (|>lseg P.t_listptr (map Vint r) y (q rho)) as B.
+ forget (field_mapsto sh list_struct P.i_h (p rho) (Vint h) ) as A.
+ forget (|>lseg P.t_listptr sh (map Vint r) y (q rho)) as B.
  erewrite (field_mapsto_typecheck_val); try reflexivity.
  normalize.
  apply prop_right.
@@ -125,15 +125,16 @@ Qed.
 
 Definition sumlist_spec :=
  DECLARE P.i_sumlist
-  WITH contents 
-  PRE [ P.i_p : P.t_listptr]  lift2 (ilseg contents) (eval_id P.i_p) (lift0 nullval)
-  POST [ P.t_int ]  local (lift1 (eq (Vint (fold_right Int.add Int.zero contents))) retval).
+  WITH sh_contents 
+  PRE [ P.i_p : P.t_listptr]  lift2 (ilseg (fst sh_contents) (snd sh_contents)) (eval_id P.i_p) (lift0 nullval)
+  POST [ P.t_int ]  local (lift1 (eq (Vint (fold_right Int.add Int.zero (snd sh_contents)))) retval).
 
 Definition reverse_spec :=
  DECLARE P.i_reverse
-  WITH contents : list int
-  PRE  [ P.i_p : P.t_listptr ] lift2 (ilseg contents) (eval_id P.i_p) (lift0 nullval)
-  POST [ P.t_listptr ] lift2 (ilseg (rev contents)) retval (lift0 nullval).
+  WITH sh_contents : share * list int
+  PRE  [ P.i_p : P.t_listptr ] !! writable_share (fst sh_contents) &&
+        lift2 (ilseg (fst sh_contents) (snd sh_contents)) (eval_id P.i_p) (lift0 nullval)
+  POST [ P.t_listptr ] lift2 (ilseg (fst sh_contents) (rev (snd sh_contents))) retval (lift0 nullval).
 
 Definition main_spec :=
  DECLARE P.i_main
@@ -151,10 +152,10 @@ Definition Gprog : funspecs :=
 Definition partial_sum (contents cts: list int) (v: val) := 
      fold_right Int.add Int.zero contents = Int.add (force_int  v) (fold_right Int.add Int.zero cts).
 
-Definition sumlist_Inv (contents: list int) : assert :=
+Definition sumlist_Inv (sh: share) (contents: list int) : assert :=
           (EX cts: list int, 
             PROP () LOCAL (lift1 (partial_sum contents cts) (eval_id P.i_s)) 
-            SEP (TT * lift2 (ilseg cts) (eval_id P.i_t) (lift0 nullval))).
+            SEP (TT * lift2 (ilseg sh cts) (eval_id P.i_t) (lift0 nullval))).
 
 Ltac start_function :=
 match goal with |- semax_body _ _ _ ?spec => try unfold spec end;
@@ -183,9 +184,10 @@ Hint Rewrite eval_expr_unop : normalize.
 Lemma body_sumlist: semax_body Vprog Gprog P.f_sumlist sumlist_spec.
 Proof.
 start_function.
+destruct sh_contents as [sh contents]. simpl @fst; simpl @snd.
 forward.
 forward.
-forward_while (sumlist_Inv contents)
+forward_while (sumlist_Inv sh contents)
     (PROP() LOCAL (lift1 (fun v => fold_right Int.add Int.zero contents = force_int v) (eval_id P.i_s))SEP(TT)).
 (* Prove that current precondition implies loop invariant *)
 unfold sumlist_Inv, partial_sum.
@@ -207,7 +209,7 @@ unfold sumlist_Inv at 1.
 autorewrite with normalize.
 apply extract_exists_pre; intro cts.
 autorewrite with normalize.
-replace_in_pre (ilseg cts) (ilseg_cons cts).
+replace_in_pre (ilseg sh cts) (ilseg_cons sh cts).
 rewrite ilseg_nonnull; auto.
 rewrite lift2_ilseg_cons.
 normalizex. intros [[h r] y].
@@ -242,21 +244,23 @@ destruct (eval_id P.i_s rho); inv H1; auto.
 unfold retval; simpl. normalize.
 Qed.
 
-Definition reverse_Inv (contents: list int) : assert :=
+Definition reverse_Inv (sh: share) (contents: list int) : assert :=
           (EX cts1: list int, EX cts2 : list int,
             PROP (contents = rev cts1 ++ cts2) 
             LOCAL ()
-            SEP (lift2 (ilseg cts1) (eval_id P.i_w) (lift0 nullval) *
-                   lift2 (ilseg cts2) (eval_id P.i_v) (lift0 nullval))).
+            SEP (lift2 (ilseg sh cts1) (eval_id P.i_w) (lift0 nullval) *
+                   lift2 (ilseg sh cts2) (eval_id P.i_v) (lift0 nullval))).
 
 Lemma body_reverse: semax_body Vprog Gprog P.f_reverse reverse_spec.
 Proof.
 start_function.
+destruct sh_contents as [sh contents]. simpl @fst; simpl @snd.
+normalizex. rename H into WS.
 forward.
 go_lower.
 forward.
-forward_while (reverse_Inv contents)
-         (PROP() LOCAL () SEP( lift2 (ilseg (rev contents)) (eval_id P.i_w) (lift0 nullval))).
+forward_while (reverse_Inv sh contents)
+         (PROP() LOCAL () SEP( lift2 (ilseg sh (rev contents)) (eval_id P.i_w) (lift0 nullval))).
 (* precondition implies loop invariant *)
 unfold reverse_Inv.
 go_lower.
@@ -279,8 +283,8 @@ apply extract_exists_pre; intro cts.
 normalize.
 apply extract_exists_pre; intro cts2.
 normalizex. subst contents.
-replace_in_pre (ilseg cts2) (ilseg_cons cts2).
-rewrite (ilseg_nonnull cts2) by auto. auto.
+replace_in_pre (ilseg sh cts2) (ilseg_cons sh cts2).
+rewrite (ilseg_nonnull sh cts2) by auto. auto.
 rewrite lift2_ilseg_cons.
 normalizex. intros [[h r] y].
 normalizex; subst cts2.
@@ -298,9 +302,9 @@ normalize.
 simpl. rewrite app_ass.
 simpl.
 normalize.
-rewrite (ilseg_unroll (h::cts)).
-apply derives_trans with (ilseg_cons (h :: cts) (eval_id P.i_w rho) nullval *
-    ilseg r (eval_id P.i_v rho) nullval).
+rewrite (ilseg_unroll sh (h::cts)).
+apply derives_trans with (ilseg_cons sh (h :: cts) (eval_id P.i_w rho) nullval *
+    ilseg sh r (eval_id P.i_v rho) nullval).
 unfold ilseg_cons, lseg_cons.
 normalize. apply exp_right with (Vint h).
 normalize. apply exp_right with (map Vint cts).
@@ -315,9 +319,9 @@ assert (eval_cast P.t_listptr P.t_listptr old_w = old_w)
   by (destruct old_w ; inv H3; simpl; auto).
 rewrite H4 in *.
 normalize.
-repeat pull_right (field_mapsto Share.top P.t_list P.i_t (eval_id P.i_w rho) old_w).
+repeat pull_right (field_mapsto sh P.t_list P.i_t (eval_id P.i_w rho) old_w).
 apply sepcon_derives; auto.
-repeat pull_right (field_mapsto Share.top list_struct P.i_h (eval_id P.i_w rho) (Vint h)).
+repeat pull_right (field_mapsto sh list_struct P.i_h (eval_id P.i_w rho) (Vint h)).
 apply sepcon_derives; auto.
 rewrite sepcon_comm.
 apply sepcon_derives; auto.
@@ -375,16 +379,102 @@ Proof.
   unfold Map.get; rewrite H4.
   destruct (H2 _ _ H1) as [b [i' [? ?]]].
    rewrite H5. simpl. rewrite eqb_type_refl.
-   simpl globtype in H6. 
-   simpl in H6. 
-   admit.  (* PROBLEM!!! Discuss with Joey *)
+   simpl globtype in H6.
+   auto. 
   destruct H4; congruence.
+Qed.
+
+Lemma tc_eval_var_nonnull:
+  forall Delta t i rho z, tc_environ Delta rho ->
+      match (var_types Delta) ! i with Some _ => True | None =>
+               match   (glob_types Delta) ! i with Some _ => True | None => False end
+      end ->
+      ~ptr_eq (eval_var i t rho) (Vint z).
+Admitted.
+
+Definition Ews (* extern_write_share *) := Share.splice extern_retainer Share.top.
+
+Lemma cast_exp_pointer2:
+  forall e t1 t2 t', typeof e = Tpointer t1 noattr -> 
+                         t' = Tpointer t2 noattr ->
+                    cast_exp e t' = eval_expr e.
+Admitted.
+
+Lemma globvar_lem1:
+  forall (ge: Genv.t fundef type) Delta rho id t,
+      tc_environ Delta rho ->
+     (var_types Delta) ! id = None ->
+     (glob_types Delta) ! id = Some  (Global_var t) ->
+     exists b, exists z,  ve_of rho id = None /\ ge_of rho id = Some (Vptr b z, t).
+Proof.
+intros.
+unfold tc_environ, typecheck_environ in H.
+repeat rewrite andb_true_iff in H. destruct H as [[[Ha Hb] Hc] Hd].
+apply environ_lemmas.typecheck_ge_eqv in Hc. 
+hnf in Hc.
+specialize (Hc _ _ H1). destruct Hc as [b [i [Hc Hc']]].
+exists b; exists i; rewrite Hc.
+split; auto.
+apply environ_lemmas.typecheck_mode_eqv in Hd.
+apply Hd in H1. 
+destruct H1; auto. destruct H; simpl in H. congruence.
+Qed.
+
+Lemma globvar2pred_lem1:
+  forall (ge: Genv.t fundef type) Delta rho id gv t,
+      tc_environ Delta rho ->
+     (glob_types Delta) ! id = Some  (Global_var t) ->
+     gvar_info gv = t ->
+     gvar_volatile gv = false ->
+      globvar2pred ge (id,gv) rho |--
+        EX b:_, EX z:_,  init_data_list2pred ge (gvar_init gv)
+                           (readonly2share (gvar_readonly gv)) b (Int.unsigned z)
+                 (ge_of rho).
+Proof.
+intros.
+unfold globvar2pred.
+simpl @fst; simpl @snd. subst t.
+unfold tc_environ, typecheck_environ in H.
+repeat rewrite andb_true_iff in H. destruct H as [[[Ha Hb] Hc] Hd].
+apply environ_lemmas.typecheck_ge_eqv in Hc. 
+hnf in Hc.
+specialize (Hc _ _ H0). destruct Hc as [b [i [Hc Hc']]]. rewrite Hc.
+rewrite H2.
+apply exp_right with b; apply exp_right with i; auto.
+Qed.
+Lemma address_field_mapsto:
+  forall ch v rsh sh b z' z ofs structid fld fields,
+  access_mode
+        (type_of_field
+           (unroll_composite_fields structid (Tstruct structid fields noattr)
+              fields) fld) = By_value ch ->
+  z' =  (Int.unsigned z + ofs)  mod Int.modulus ->
+  field_offset fld fields = Errors.OK ofs ->
+  (typecheck_val v
+         (type_of_field
+            (unroll_composite_fields structid
+               (Tstruct structid fields noattr) fields) fld) = true)  ->
+  (type_is_volatile
+         (type_of_field
+            (unroll_composite_fields structid
+               (Tstruct structid fields noattr) fields) fld) = false) ->
+  address_mapsto ch v rsh sh (b, z') |--
+  field_mapsto (Share.splice rsh sh) (Tstruct structid fields noattr) fld (Vptr b z) v.
+Proof.
+ intros.
+ Transparent field_mapsto. unfold field_mapsto.
+  simpl. rewrite field_offset_unroll. rewrite H1. rewrite H.
+  normalize.
+  subst.
+ rewrite Zplus_mod_idemp_r. 
+ rewrite Share.unrel_splice_L. rewrite Share.unrel_splice_R.
+ auto. Opaque field_mapsto.
 Qed.
 
 Lemma setup_globals:
   forall rho,  tc_environ (func_tycontext P.f_main Vprog Gprog) rho ->
    main_pre P.prog tt rho
-   |-- ilseg (Int.repr 1 :: Int.repr 2 :: Int.repr 3 :: nil)
+   |-- ilseg Ews (Int.repr 1 :: Int.repr 2 :: Int.repr 3 :: nil)
       (cast_exp
          (Ecast
             (Eaddrof (Evar P.i_three (Tarray P.t_list 3 noattr))
@@ -392,16 +482,127 @@ Lemma setup_globals:
          P.t_listptr rho) nullval * fold_right sepcon emp nil rho.
 Proof.
  unfold main_pre.
- go_lower. unfold P.prog, globvars2pred. simpl.
-   unfold globvar2pred; simpl.
+ go_lower.
+ destruct (globvar_lem1 (Genv.globalenv P.prog) _ _ P.i_three _ H (eq_refl _) (eq_refl _)) 
+    as [b [z [H98 H99]]]. simpl in H99.
+ assert (H97: eval_var P.i_three (Tarray P.t_list 3 noattr) rho = Vptr b z).
+  unfold eval_var. unfold Map.get. rewrite H98; rewrite H99. rewrite eqb_type_refl; auto.
+ unfold P.prog, globvars2pred. simpl.
+  unfold globvar2pred.
+ normalize. simpl. rewrite H99.
    unfold ilseg.
   rewrite lseg_unroll. apply orp_right2. unfold lseg_cons.
   rewrite prop_true_andp.
 Focus 2.
   erewrite cast_exp_pointer by reflexivity.
   normalize. simpl eval_cast.
-Admitted.  (* Needs work *)
+ rewrite eval_cast_pointer; simpl; auto; try solve [eapply tc_eval_gvar_i; eauto].
+ eapply tc_eval_var_nonnull; eauto.  compute; auto.
+  (* End Focus 2 *)
+  apply exp_right with (Vint (Int.repr 1)).
+  apply exp_right with (Vint (Int.repr 2)::Vint (Int.repr 3)::nil).
+  apply exp_right with (eval_expr (Ebinop Cop.Oadd 
+                                    (Eaddrof (Evar P.i_three (Tarray P.t_list 3 noattr)) P.t_listptr)
+                                    (Econst_int (Int.repr 1) P.t_int)  P.t_listptr) rho).
+ simpl. normalize.
+ rewrite prop_true_andp.
+2:   admit.  (* typechecking proof *)
+  rewrite sepcon_assoc.
+  apply sepcon_derives.
+ erewrite cast_exp_pointer2; [ | reflexivity | reflexivity].
+ normalize. 
+ erewrite eval_cast_pointer; [ | compute; auto| eapply tc_eval_gvar_i; eauto ].
+ simpl eval_expr. rewrite H97.
+ unfold list_struct.
+ apply address_field_mapsto with 0; simpl; try solve [rewrite if_true; auto].
+ admit.  (* easy *)
+ unfold field_offset. simpl. rewrite if_true; auto.
+ apply sepcon_derives.
+ erewrite cast_exp_pointer2; [ | reflexivity | reflexivity].
+ normalize. 
+ erewrite eval_cast_pointer; [ | compute; auto| eapply tc_eval_gvar_i; eauto ].
+ simpl eval_expr.  rewrite H97.
+ apply address_field_mapsto with 4; simpl;
+   repeat rewrite if_false by (intro Hx; inv Hx); repeat rewrite if_true by auto; auto.
+ admit.  (* perhaps provable from structure of initializers *)
+ unfold field_offset. simpl.
+   repeat rewrite if_false by (intro Hx; inv Hx); repeat rewrite if_true by auto; auto.
 
+  eapply derives_trans; [ | apply now_later].
+  rewrite lseg_unroll. apply orp_right2. unfold lseg_cons.
+  rewrite prop_true_andp.
+  2: admit.  (* like the one above *)
+  apply exp_right with (Vint (Int.repr 2)).
+  apply exp_right with (Vint (Int.repr 3)::nil).
+  apply exp_right with (eval_expr (Ebinop Cop.Oadd 
+                                    (Eaddrof (Evar P.i_three (Tarray P.t_list 3 noattr)) P.t_listptr)
+                                    (Econst_int (Int.repr 2) P.t_int)  P.t_listptr) rho).
+ simpl. normalize.
+ rewrite prop_true_andp.
+2:   admit.  (* typechecking proof *)
+  rewrite sepcon_assoc.
+  apply sepcon_derives.  rewrite H97.
+ unfold eval_binop. simpl. repeat rewrite Zmax_spec; simpl.
+ unfold align. simpl.
+  rewrite Int.mul_signed. repeat rewrite Int.signed_repr. simpl.
+ apply address_field_mapsto with 0; simpl; try solve [rewrite if_true; auto].
+  admit.  (* perhaps provable from structure of initializers *)
+ unfold field_offset. simpl.
+   repeat rewrite if_false by (intro Hx; inv Hx); repeat rewrite if_true by auto; auto.
+ admit.  (* easy *)
+ admit.  (* easy *)
+  apply sepcon_derives.  rewrite H97.
+ unfold eval_binop. simpl. repeat rewrite Zmax_spec; simpl.
+ unfold align. simpl.
+  rewrite Int.mul_signed. repeat rewrite Int.signed_repr. simpl.
+ apply address_field_mapsto with 4; simpl;
+   repeat rewrite if_false by (intro Hx; inv Hx); repeat rewrite if_true by auto; auto.
+ admit. 
+ unfold field_offset. simpl.
+   repeat rewrite if_false by (intro Hx; inv Hx); repeat rewrite if_true by auto; auto.
+ admit.  (* easy *)
+ admit.  (* easy *)
+  eapply derives_trans; [ | apply now_later].
+  rewrite lseg_unroll. apply orp_right2. unfold lseg_cons.
+  rewrite prop_true_andp.
+  2: admit.  (* like the one above *)
+  apply exp_right with (Vint (Int.repr 3)).
+  apply exp_right with (nil).
+  apply exp_right with nullval.
+ simpl. normalize.
+ match goal with |- ?A |-- sepcon ?B ?C => apply derives_trans with (B*emp) end.
+ rewrite sepcon_emp.
+  apply sepcon_derives. rewrite H97.
+ unfold eval_binop. simpl. repeat rewrite Zmax_spec; simpl.
+ unfold align. simpl.
+  rewrite Int.mul_signed. repeat rewrite Int.signed_repr. simpl.
+ apply address_field_mapsto with 0; simpl; try solve [rewrite if_true; auto].
+  admit.  (* perhaps provable from structure of initializers *)
+ unfold field_offset. simpl.
+   repeat rewrite if_false by (intro Hx; inv Hx); repeat rewrite if_true by auto; auto.
+ admit.  (* easy *)
+ admit.  (* easy *)
+ rewrite H97.
+ unfold eval_binop. simpl. repeat rewrite Zmax_spec; simpl.
+ unfold align. simpl.
+  rewrite Int.mul_signed. repeat rewrite Int.signed_repr. simpl.
+ apply address_field_mapsto with 4; simpl;
+   repeat rewrite if_false by (intro Hx; inv Hx); repeat rewrite if_true by auto; auto.
+ admit. 
+ unfold field_offset. simpl.
+   repeat rewrite if_false by (intro Hx; inv Hx); repeat rewrite if_true by auto; auto.
+ admit.  (* easy *)
+ admit.  (* easy *)
+  apply sepcon_derives; auto.
+  eapply derives_trans; [ | apply now_later].
+  rewrite lseg_unroll. apply orp_right1.
+  rewrite prop_true_andp. normalize.
+  unfold ptr_eq. simpl. rewrite Int.eq_true; auto.
+Qed.
+
+Lemma writable_Ews: writable_share Ews.
+Admitted.
+Hint Resolve writable_Ews.
 
 Lemma body_main:  semax_body Vprog Gprog P.f_main main_spec.
 Proof.
@@ -409,19 +610,22 @@ start_function.
 normalize.
 forward. 
 go_lower. unfold F,x.
-instantiate (2:= (Int.repr 1 :: Int.repr 2 :: Int.repr 3 :: nil)).
+instantiate (2:= (Ews, Int.repr 1 :: Int.repr 2 :: Int.repr 3 :: nil)).
 instantiate (1:=nil).
 rewrite prop_true_andp by (compute; intuition).
+rewrite prop_true_andp by auto.
 destruct u; apply setup_globals; auto.
 unfold x,F in *; clear x F.
 apply extract_exists_pre; normalize.
 forward.
 go_lower. 
 unfold x,F.
-instantiate (2:= (Int.repr 3 :: Int.repr 2 :: Int.repr 1 :: nil)).
+instantiate (2:= (Ews, Int.repr 3 :: Int.repr 2 :: Int.repr 1 :: nil)).
 instantiate (1:=nil).
 normalize.
-admit.
+rewrite prop_true_andp by (compute; auto).
+erewrite cast_exp_pointer by reflexivity.
+normalize.
 apply extract_exists_pre; intro old.
 normalize. clear old.
 forward.
